Kami/Ex/ProcDecInv.v
@@ -9,6 +9,8 @@ Require Import Eqdep ProofIrrelevance.
 
 Set Implicit Arguments.
 
+Local Hint Unfold listIsEmpty listEnq listDeq listFirstElt: MethDefs.
+
 Lemma wnot_not_zero_wplusone:
   forall {sz} (w2: word sz),
     wnot w2 <> $0 ->
@@ -55,7 +57,7 @@ Proof.
 Qed.
 
 Section Invariants.
-  Variables addrSize iaddrSize fifoSize instBytes dataBytes rfIdx: nat.
+  Variables addrSize iaddrSize instBytes dataBytes rfIdx: nat.
 
   Variables (fetch: AbsFetch addrSize iaddrSize instBytes dataBytes)
             (dec: AbsDec addrSize instBytes dataBytes rfIdx)
@@ -66,70 +68,72 @@ Section Invariants.
 
   Variable (init: ProcInit iaddrSize dataBytes rfIdx).
 
-  Definition pdecInl := pdecInl fifoSize fetch dec exec init.
+  Definition pdecInl := projT1 (pdecInl fetch dec exec init).
 
-  Definition fifoLength (emptyv fullv: bool)
-             (enqpv deqpv: type (Bit fifoSize)) :=
-    if emptyv then 0
-    else if fullv then NatLib.pow2 fifoSize
-         else #(enqpv ^- deqpv).
+  Fixpoint pgm_init_rq_inv
+           (pinitRqv: type Bool)
+           (pinitRqOfsv: type (Bit iaddrSize))
+           (ieltv: listEltT (Struct RqFromProc) type) :=
+    match ieltv with
+    | nil => True
+    | rq :: rqs =>
+      rq = evalExpr
+             (STRUCT { "addr" ::=
+                         alignAddr _ (natToWord _ ((if pinitRqv
+                                                    then NatLib.pow2 iaddrSize
+                                                    else wordToNat pinitRqOfsv)
+                                                   - List.length ieltv));
+                       "op" ::= $$false;
+                       "data" ::= $0 })%kami_expr /\
+      pgm_init_rq_inv pinitRqv pinitRqOfsv rqs
+    end.
 
-  Definition fifo_inv (emptyv fullv: bool)
-             (enqpv deqpv: type (Bit fifoSize)): Prop :=
-    (emptyv || fullv = true <-> enqpv = deqpv).
-
-  Definition fifo_rq_rs_inv
+  Definition pgm_init_rq_rs_inv
              (pinitRqv: type Bool)
              (pinitRqOfsv pinitRsOfsv: type (Bit iaddrSize))
-             (iemptyv ifullv oemptyv ofullv: type Bool)
-             (ienqpv ideqpv oenqpv odeqpv: type (Bit fifoSize)) :=
-    fifo_inv iemptyv ifullv ienqpv ideqpv /\
-    fifo_inv oemptyv ofullv oenqpv odeqpv /\
-    (if pinitRqv then NatLib.pow2 iaddrSize
-     else #pinitRqOfsv) =
-    #pinitRsOfsv +
-    fifoLength iemptyv ifullv ienqpv ideqpv +
-    fifoLength oemptyv ofullv oenqpv odeqpv.
+             (ieltv: listEltT (Struct RqFromProc) type)
+             (oeltv: listEltT (Struct RsToProc) type) :=
+    (if pinitRqv then NatLib.pow2 iaddrSize else #pinitRqOfsv) =
+    #pinitRsOfsv + List.length ieltv + List.length oeltv.
 
-  Definition fifo_empty_inv (fifoEmpty: bool) (fifoEnqP fifoDeqP: type (Bit fifoSize)): Prop :=
-    fifoEmpty = true /\ fifoEnqP = fifoDeqP.
+  Definition fifo_empty_inv {k: Kind} (eltv: listEltT k type) :=
+    eltv = nil.
   
-  Definition fifo_not_empty_inv (fifoEmpty: bool) (fifoEnqP fifoDeqP: type (Bit fifoSize)): Prop :=
-    fifoEmpty = false /\ fifoEnqP = fifoDeqP ^+ $1.
+  Definition fifo_not_empty_inv {k: Kind} (eltv: listEltT k type) :=
+    List.length eltv = 1.
 
   Definition mem_request_inv
              (rawInst: fullType type (SyntaxKind (Data instBytes)))
              (rf: fullType type (SyntaxKind (Vector (Data dataBytes) rfIdx)))
-             (insEmpty: bool) (insElt: type (Vector (Struct RqFromProc) fifoSize))
-             (insDeqP: type (Bit fifoSize)): Prop.
+             (insElt: listEltT (Struct RqFromProc) type): Prop.
   Proof.
-    refine (if insEmpty then True else _).
+    destruct insElt as [|rq rqs]; [exact True|].
     refine (_ /\ _).
-    - exact ((insElt insDeqP (RqFromProc !! "op") = false ->
+    - exact ((rq (RqFromProc !! "op") = false ->
               evalExpr (getOptype _ rawInst) = opLd) /\
              (evalExpr (getOptype _ rawInst) = opLd ->
-              (insElt insDeqP (RqFromProc !! "op") = false /\
-               insElt insDeqP (RqFromProc !! "addr") =
+              (rq (RqFromProc !! "op") = false /\
+               rq (RqFromProc !! "addr") =
                evalExpr
                  (alignLdAddr
                     _ (evalExpr
                          (calcLdAddr
                             _ (evalExpr (getLdAddr _ rawInst))
                             (evalExpr (#rf@[getLdSrc _ rawInst])%kami_expr)))) /\
-               insElt insDeqP (RqFromProc !! "data") =
+               rq (RqFromProc !! "data") =
                evalConstT (getDefaultConst (Data dataBytes))))).
-    - exact ((insElt insDeqP (RqFromProc !! "op") = true ->
+    - exact ((rq (RqFromProc !! "op") = true ->
               evalExpr (getOptype _ rawInst) = opSt) /\
              (evalExpr (getOptype _ rawInst) = opSt ->
-              (insElt insDeqP (RqFromProc !! "op") = true /\
-               insElt insDeqP (RqFromProc !! "addr") =
+              (rq (RqFromProc !! "op") = true /\
+               rq (RqFromProc !! "addr") =
                evalExpr (calcStAddr
                            _ (evalExpr (getStAddr _ rawInst))
                            (evalExpr (#rf@[getStSrc _ rawInst])%kami_expr)) /\
-               insElt insDeqP (RqFromProc !! "data") =
+               rq (RqFromProc !! "data") =
                evalExpr (#rf@[getStVSrc _ rawInst ])%kami_expr))).
   Defined.
-  Hint Unfold fifo_rq_rs_inv fifo_inv fifo_empty_inv fifo_not_empty_inv
+  Hint Unfold pgm_init_rq_rs_inv fifo_empty_inv fifo_not_empty_inv
        mem_request_inv: InvDefs.
 
   Record procDec_inv (o: RegsT) : Prop :=
@@ -151,43 +155,22 @@ Section Invariants.
       Hpgmv : M.find "pgm"%string o = Some (existT _ _ pgmv);
       stallv : fullType type (SyntaxKind Bool);
       Hstallv : M.find "stall"%string o = Some (existT _ _ stallv);
-      iev : fullType type (SyntaxKind Bool);
-      Hiev : M.find "rqFromProc"--"empty"%string o = Some (existT _ _ iev);
-      ifv : fullType type (SyntaxKind Bool);
-      Hifv : M.find "rqFromProc"--"full"%string o = Some (existT _ _ ifv);
-      ienqpv : fullType type (SyntaxKind (Bit fifoSize));
-      Hienqpv : M.find "rqFromProc"--"enqP"%string o = Some (existT _ _ ienqpv);
-      ideqpv : fullType type (SyntaxKind (Bit fifoSize));
-      Hideqpv : M.find "rqFromProc"--"deqP"%string o = Some (existT _ _ ideqpv);
-      ieltv : fullType type (SyntaxKind (Vector (Struct RqFromProc) fifoSize));
+
+      ieltv : fullType type (listEltK (Struct RqFromProc) type);
       Hieltv : M.find "rqFromProc"--"elt"%string o = Some (existT _ _ ieltv);
-      oev : fullType type (SyntaxKind Bool);
-      Hoev : M.find "rsToProc"--"empty"%string o = Some (existT _ _ oev);
-      ofv : fullType type (SyntaxKind Bool);
-      Hofv : M.find "rsToProc"--"full"%string o = Some (existT _ _ ofv);
-      oenqpv : fullType type (SyntaxKind (Bit fifoSize));
-      Hoenqpv : M.find "rsToProc"--"enqP"%string o = Some (existT _ _ oenqpv);
-      odeqpv : fullType type (SyntaxKind (Bit fifoSize));
-      Hodeqpv : M.find "rsToProc"--"deqP"%string o = Some (existT _ _ odeqpv);
-      oeltv : fullType type (SyntaxKind (Vector (Struct RsToProc) fifoSize));
+      oeltv : fullType type (listEltK (Struct RsToProc) type);
       Hoeltv : M.find "rsToProc"--"elt"%string o = Some (existT _ _ oeltv);
 
       Hinv :
         (pinitv = false ->
-         fifo_rq_rs_inv pinitRqv pinitRqOfsv pinitRsOfsv
-                        iev ifv oev ofv ienqpv ideqpv oenqpv odeqpv /\
+         pgm_init_rq_inv pinitRqv pinitRqOfsv ieltv /\
+         pgm_init_rq_rs_inv pinitRqv pinitRqOfsv pinitRsOfsv ieltv oeltv /\
          stallv = false) /\
         (pinitv = true ->
-         or3 (stallv = false /\
-              fifo_empty_inv iev ienqpv ideqpv /\
-              fifo_empty_inv oev oenqpv odeqpv)
-             ((stallv = true /\
-               fifo_not_empty_inv iev ienqpv ideqpv /\
-               fifo_empty_inv oev oenqpv odeqpv) /\
-              (mem_request_inv (pgmv (split2 _ _ pcv)) rfv iev ieltv ideqpv))
-             (stallv = true /\
-              fifo_empty_inv iev ienqpv ideqpv /\
-              fifo_not_empty_inv oev oenqpv odeqpv))
+         or3 (stallv = false /\ fifo_empty_inv ieltv /\ fifo_empty_inv oeltv)
+             ((stallv = true /\ fifo_not_empty_inv ieltv /\ fifo_empty_inv oeltv) /\
+              (mem_request_inv (pgmv (split2 _ _ pcv)) rfv ieltv))
+             (stallv = true /\ fifo_empty_inv ieltv /\ fifo_not_empty_inv oeltv))
         }.
 
   Ltac procDec_inv_old :=
@@ -212,219 +195,120 @@ Section Invariants.
     | 2 => or3_thd (* responded *)
     end; intuition idtac.
 
-  Lemma fifoLength_enq:
-    forall emptyv enqpv deqpv,
-      fifo_inv emptyv false enqpv deqpv ->
-      fifoLength emptyv false enqpv deqpv + 1 =
-      fifoLength false (if weq deqpv (enqpv ^+ $1) then true else false)
-                 (enqpv ^+ $1) deqpv.
+  Lemma pgm_init_rq_inv_enq_not_last:
+    forall elts rqOfs,
+      wnot rqOfs <> $0 ->
+      pgm_init_rq_inv false rqOfs elts ->
+      forall elt,
+        elt = evalExpr
+                (STRUCT { "addr" ::= alignAddr _ rqOfs;
+                          "op" ::= $$false;
+                          "data" ::= $0})%kami_expr ->
+        pgm_init_rq_inv false (rqOfs ^+ $1) (listEnq elt elts).
   Proof.
-    unfold fifo_inv, fifoLength; intros.
-    destruct H.
-    destruct emptyv; simpl in *.
-    - specialize (H eq_refl); subst.
-      destruct (weq deqpv (deqpv ^+ $1)).
-      + destruct fifoSize; [reflexivity|].
-        exfalso; eapply wplus_one_neq; eauto.
-      + rewrite wminus_def, <-wplus_assoc.
-        rewrite wplus_comm with (x:= $1).
-        rewrite wplus_assoc.
-        rewrite wminus_inv, wplus_wzero_2.
-        destruct fifoSize.
-        * elim n.
-          rewrite (word0 deqpv); reflexivity.
-        * rewrite roundTrip_1; reflexivity.
-    - destruct (weq deqpv (enqpv ^+ $1)); subst.
-      + rewrite wminus_def, wneg_wplus_distr.
-        rewrite wplus_assoc, wminus_inv, wplus_wzero_2.
-        destruct fifoSize; [reflexivity|].
-        rewrite <-wones_wneg_one.
-        rewrite wones_pow2_minus_one.
-        pose proof (NatLib.pow2_zero (S n)); omega.
-      + rewrite wminus_def with (x:= enqpv ^+ _).
-        rewrite <-wplus_assoc, wplus_comm with (x:= $1).
-        rewrite wplus_assoc, <-wminus_def.
-        erewrite wordToNat_plusone with (w':= wones _).
-        * omega.
-        * apply lt_wlt.
-          pose proof (wordToNat_bound (enqpv ^- deqpv)).
-          rewrite wones_pow2_minus_one.
-          assert (#(enqpv ^- deqpv) <> NatLib.pow2 fifoSize - 1).
-          { intro Hx.
-            rewrite <-wones_pow2_minus_one in Hx.
-            assert (enqpv ^- deqpv = wones fifoSize).
-            { rewrite <-natToWord_wordToNat, <-Hx.
-              rewrite natToWord_wordToNat; reflexivity.
-            }
-            assert (^~ (enqpv ^- deqpv) = $1).
-            { rewrite H2, <-wneg_idempotent with (w:= $1).
-              rewrite wones_wneg_one; reflexivity.
-            }
-            elim n.
-            rewrite <-H3.
-            rewrite wminus_def, wneg_wplus_distr.
-            rewrite wplus_assoc, wneg_idempotent.
-            rewrite wminus_inv, wplus_wzero_2.
-            reflexivity.
-          }
-          omega.
+    induction elts; intros.
+    - simpl; split; auto.
+      rewrite H1; simpl; kinv_eq.
+      rewrite wnot_not_zero_wplusone by assumption.
+      rewrite Nat.add_sub.
+      rewrite natToWord_wordToNat.
+      reflexivity.
+    - simpl in H0; dest; subst.
+      split.
+      + simpl; kinv_eq.
+        rewrite app_length; simpl.
+        rewrite wnot_not_zero_wplusone by assumption.
+        do 3 f_equal; omega.
+      + apply IHelts; auto.
   Qed.
 
-  Lemma fifoLength_deq:
-    forall fullv enqpv deqpv,
-      fifo_inv false fullv enqpv deqpv ->
-      fifoLength false fullv enqpv deqpv =
-      fifoLength (if weq enqpv (deqpv ^+ $1) then true else false) false 
-                 enqpv (deqpv ^+ $1) + 1.
+  Lemma pgm_init_rq_inv_enq_last:
+    forall elts rqOfs,
+      wnot rqOfs = $0 ->
+      pgm_init_rq_inv false rqOfs elts ->
+      forall elt,
+        elt = evalExpr
+                (STRUCT { "addr" ::= alignAddr _ rqOfs;
+                          "op" ::= $$false;
+                          "data" ::= $0})%kami_expr ->
+        pgm_init_rq_inv true $0 (listEnq elt elts).
   Proof.
-    unfold fifo_inv, fifoLength; intros.
-    destruct H.
-    destruct fullv; simpl in *.
-    - specialize (H eq_refl); subst.
-      destruct (weq deqpv (deqpv ^+ $1)).
-      + destruct fifoSize; [reflexivity|].
-        exfalso; eapply wplus_one_neq; eauto.
-      + rewrite wminus_def, wneg_wplus_distr.
-        rewrite wplus_assoc, wminus_inv, wplus_wzero_2.
-        rewrite <-wones_wneg_one.
-        rewrite wones_pow2_minus_one.
-        pose proof (NatLib.pow2_zero fifoSize); omega.
-    - destruct (weq enqpv (deqpv ^+ $1)).
-      + subst.
-        rewrite wminus_def, <-wplus_assoc.
-        rewrite wplus_comm with (x:= $1).
-        rewrite wplus_assoc.
-        rewrite wminus_inv, wplus_wzero_2.
-        destruct fifoSize.
-        * rewrite (word0 deqpv) in H0.
-          specialize (H0 eq_refl); discriminate.
-        * rewrite roundTrip_1; reflexivity.
-      + rewrite wminus_plus_distr.
-        rewrite <-wordToNat_minus_one'.
-        * omega.
-        * intro Hx.
-          apply sub_0_eq in Hx; subst.
-          specialize (H0 eq_refl); discriminate.
+    induction elts; intros.
+    - simpl; split; auto.
+      rewrite H1; simpl; kinv_eq.
+      rewrite wnot_zero_wones with (w:= rqOfs) by assumption.
+      rewrite wones_natToWord; reflexivity.
+    - simpl in H0; dest; subst.
+      split.
+      + simpl; kinv_eq.
+        rewrite app_length; simpl.
+        rewrite wnot_zero_wones with (w:= rqOfs) by assumption.
+        rewrite wones_natToWord.
+        do 3 f_equal.
+        pose proof (NatLib.pow2_zero iaddrSize).
+        rewrite wordToNat_natToWord_2; omega.
+      + apply IHelts; auto.
   Qed.
 
-  Lemma fifoLength_zero:
-    forall emptyv fullv enqpv deqpv,
-      fifo_inv emptyv fullv enqpv deqpv ->
-      fifoLength emptyv fullv enqpv deqpv = 0 ->
-      emptyv = true /\ enqpv = deqpv.
+  Lemma pgm_init_rq_inv_deq:
+    forall elts rqf rqOfs,
+      pgm_init_rq_inv rqf rqOfs elts ->
+      pgm_init_rq_inv rqf rqOfs (listDeq elts).
   Proof.
-    unfold fifo_inv, fifoLength; intros.
-    destruct emptyv.
-    - destruct H; specialize (H eq_refl); subst; auto.
-    - destruct fullv.
-      + pose proof (NatLib.pow2_zero fifoSize); omega.
-      + exfalso.
-        rewrite <-wordToNat_wzero with (sz:= fifoSize) in H0.
-        assert (enqpv ^- deqpv = wzero fifoSize).
-        { rewrite <-natToWord_wordToNat, <-H0.
-          rewrite natToWord_wordToNat.
-          reflexivity.
-        }
-        apply sub_0_eq in H1; subst.
-        destruct H; specialize (H1 eq_refl); discriminate.
+    induction elts; intros; auto.
+    simpl in H; dest; subst.
+    simpl; assumption.
   Qed.
 
-  Lemma fifoLength_one:
-    forall fullv enqpv deqpv,
-      fifo_inv false fullv enqpv deqpv ->
-      fifoLength false fullv enqpv deqpv = 1 ->
-      fifoSize = 0 \/ enqpv = deqpv ^+ $1.
-  Proof.
-    unfold fifo_inv, fifoLength; intros.
-    destruct fifoSize; [left; reflexivity|].
-    destruct fullv.
-    - exfalso; pose proof (NatLib.one_lt_pow2 n); omega.
-    - right.
-      rewrite wplus_comm.
-      apply wminus_wplus_transpose.
-      rewrite <-natToWord_wordToNat with (w:= enqpv ^- deqpv).
-      congruence.
-  Qed.
-
-  Lemma fifoLength_not_empty:
-    forall fullv enqpv deqpv,
-      fifo_inv false fullv enqpv deqpv ->
-      (fifoLength false fullv enqpv deqpv > 0)%nat.
-  Proof.
-    unfold fifo_inv, fifoLength; intros.
-    destruct fullv.
-    - apply NatLib.pow2_zero.
-    - apply gt0_wneq0.
-      intro Hx.
-      apply wminus_wplus_transpose in Hx.
-      rewrite wplus_wzero_2 in Hx; subst.
-      destruct H; specialize (H0 eq_refl).
-      discriminate.
-  Qed.
-
-  Lemma fifo_rq_rs_inv_last:
+  Lemma pgm_init_rq_rs_inv_last:
     forall (pinitRqv: type Bool) (pinitRqOfsv: type (Bit iaddrSize))
-           iev ifv ienqpv ideqpv ofv oenqpv odeqpv,
-      fifo_inv iev ifv ienqpv ideqpv ->
-      fifo_inv false ofv oenqpv odeqpv ->
+           (ieltv: listEltT (Struct RqFromProc) type)
+           (oeltv: listEltT (Struct RsToProc) type),
+      oeltv <> nil ->
       (if pinitRqv then NatLib.pow2 iaddrSize else # (pinitRqOfsv)) =
-      (NatLib.pow2 iaddrSize - 1) +
-      fifoLength iev ifv ienqpv ideqpv +
-      fifoLength false ofv oenqpv odeqpv ->
-      pinitRqv = true /\
-      iev = true /\ (* ifv = false /\ *) ienqpv = ideqpv /\
-      oenqpv = odeqpv ^+ $1.
+      NatLib.pow2 iaddrSize - 1 + Datatypes.length ieltv + Datatypes.length oeltv ->
+      pinitRqv = true /\ ieltv = nil /\ List.length oeltv = 1.
   Proof.
     intros.
-    pose proof (fifoLength_not_empty H0).
-    find_if_inside;
-      [|exfalso; pose proof (wordToNat_bound pinitRqOfsv); omega].
-
-    assert (fifoLength iev ifv ienqpv ideqpv = 0) by omega.
-    apply fifoLength_zero in H3; [|assumption].
-    dest; subst.
-
-    assert (fifoLength false ofv oenqpv odeqpv = 1) by omega.
-    apply fifoLength_one in H3; [|assumption].
-    destruct H3.
-    - clear -H3; subst.
-      repeat split.
-      rewrite (word0 oenqpv), (word0 odeqpv); reflexivity.
-    - subst; repeat split.
+    find_if_inside.
+    - destruct oeltv; [exfalso; auto|].
+      destruct ieltv; simpl in H0; [|omega].
+      destruct oeltv; simpl in H0; [|omega].
+      auto.
+    - destruct oeltv; [exfalso; auto|].
+      simpl in H0.
+      exfalso.
+      pose proof (wordToNat_bound pinitRqOfsv); omega.
   Qed.
 
   Lemma procDec_inv_ok':
     forall init n ll,
-      init = initRegs (getRegInits (fst pdecInl)) ->
-      Multistep (fst pdecInl) init n ll ->
+      init = initRegs (getRegInits pdecInl) ->
+      Multistep pdecInl init n ll ->
       procDec_inv n.
   Proof. (* SKIP_PROOF_OFF *)
     induction 2.
 
     - kinv_dest_custom procDec_inv_tac.
       kinv_constr.
+      + simpl; auto.
       + cbn; repeat rewrite wordToNat_wzero; split; intros; reflexivity.
-      + cbn; repeat rewrite wordToNat_wzero; split; intros; reflexivity.
-      + cbn; repeat rewrite wordToNat_wzero; reflexivity.
       + procDec_inv_next 0.
 
     - kinvert; [mred|mred|..].
       + kinv_dest_custom procDec_inv_tac; kinv_constr.
-        * split; intros.
-          { rewrite orb_false_l in H2; find_if_inside; [auto|discriminate]. }
-          { rewrite orb_false_l; find_if_inside; [reflexivity|exfalso; auto]. }
-        * assumption.
-        * rewrite wnot_not_zero_wplusone by assumption.
-          erewrite <-fifoLength_enq with (emptyv:= iev) by (apply H; auto).
+        * kinv_regmap_red.
+          apply pgm_init_rq_inv_enq_not_last; auto.
+        * kinv_regmap_red.
+          rewrite app_length; simpl in *.
+          rewrite wnot_not_zero_wplusone by assumption.
           omega.
 
       + kinv_dest_custom procDec_inv_tac; kinv_constr.
-        * split; intros.
-          { rewrite orb_false_l in H2; find_if_inside; [auto|discriminate]. }
-          { rewrite orb_false_l; find_if_inside; [reflexivity|exfalso; auto]. }
-        * assumption.
-        * erewrite <-fifoLength_enq with (emptyv:= iev) by (apply H; auto).
-          replace #x1 with (NatLib.pow2 iaddrSize - 1) in H4.
+        * eapply pgm_init_rq_inv_enq_last; eauto.
+        * kinv_regmap_red.
+          rewrite app_length; simpl in *.
+          replace #x1 with (NatLib.pow2 iaddrSize - 1) in H2.
           { pose proof (NatLib.pow2_zero iaddrSize); omega. }
           { replace x1 with (wones iaddrSize).
             { apply eq_sym, wones_pow2_minus_one. }
@@ -433,53 +317,67 @@ Section Invariants.
 
       + kinv_dest_custom procDec_inv_tac; kinv_constr.
         * assumption.
-        * split; intros.
-          { rewrite orb_false_r in H2; find_if_inside; [auto|discriminate]. }
-          { rewrite orb_false_r; find_if_inside; [reflexivity|exfalso; auto]. }
-        * rewrite wnot_not_zero_wplusone by assumption.
-          rewrite fifoLength_deq in H4 by (apply H3; auto).
-          omega.
-          
-      + kinv_dest_custom procDec_inv_tac; kinv_constr.
-        apply wnot_zero_wones in e; subst.
-        rewrite wones_pow2_minus_one in H4.
-        eapply fifo_rq_rs_inv_last in H4; [|assumption|assumption].
-        dest; subst.
-        procDec_inv_next 0; kinv_finish.
+        * kinv_regmap_red.
+          rewrite wnot_not_zero_wplusone by assumption.
+          destruct x1; [discriminate|].
+          simpl in *; omega.
 
       + kinv_dest_custom procDec_inv_tac; kinv_constr.
-        procDec_inv_next 1; kinv_eq; kinv_finish.
+        apply wnot_zero_wones in e; subst.
+        rewrite wones_pow2_minus_one in H2.
+        eapply pgm_init_rq_rs_inv_last in H2; [|destruct x1; discriminate].
+        dest; subst.
+        destruct x1; [discriminate|].
+        destruct x1; [|discriminate].
+        procDec_inv_next 0.
+
       + kinv_dest_custom procDec_inv_tac; kinv_constr.
-        procDec_inv_next 1; kinv_eq; kinv_finish.
+        procDec_inv_next 1; kinv_eq.
+        simpl; kinv_constr; kinv_finish.
+      + kinv_dest_custom procDec_inv_tac; kinv_constr.
+        procDec_inv_next 1; kinv_eq.
+        simpl; kinv_constr; kinv_finish.
+      + kinv_dest_custom procDec_inv_tac; kinv_constr.
+        procDec_inv_next 0.
+        destruct x; [discriminate|].
+        destruct x; [reflexivity|discriminate].
+      + kinv_dest_custom procDec_inv_tac; kinv_constr.
+        procDec_inv_next 0.
+        destruct x; [discriminate|].
+        destruct x; [reflexivity|discriminate].
+      + kinv_dest_custom procDec_inv_tac; kinv_constr.
+        procDec_inv_next 0.
+        destruct x; [discriminate|].
+        destruct x; [reflexivity|discriminate].
       + kinv_dest_custom procDec_inv_tac; kinv_constr.
         procDec_inv_next 0.
       + kinv_dest_custom procDec_inv_tac; kinv_constr.
         procDec_inv_next 0.
+
       + kinv_dest_custom procDec_inv_tac; kinv_constr.
-        procDec_inv_next 0.
-      + kinv_dest_custom procDec_inv_tac; kinv_constr.
-        procDec_inv_next 0.
-      + kinv_dest_custom procDec_inv_tac; kinv_constr.
-        procDec_inv_next 0.
-      + kinv_dest_custom procDec_inv_tac; kinv_constr.
-        * split; intros.
-          { rewrite orb_false_r in H2; find_if_inside; [assumption|discriminate]. }
-          { rewrite orb_false_r; find_if_inside; [reflexivity|exfalso; auto]. }
-        * split; intros.
-          { rewrite orb_false_l in H2; find_if_inside; [auto|discriminate]. }
-          { rewrite orb_false_l; find_if_inside; [reflexivity|exfalso; auto]. }
-        * erewrite <-fifoLength_enq with (emptyv:= oev) by assumption.
-          rewrite Nat.add_comm with (m:= 1), Nat.add_assoc.
-          rewrite <-Nat.add_assoc with (n:= #pinitRsOfsv).
-          erewrite <-fifoLength_deq with (fullv:= ifv) by assumption.
-          assumption.
+        * apply pgm_init_rq_inv_deq; assumption.
+        * rewrite H2.
+          destruct x; [discriminate|].
+          kinv_regmap_red.
+          rewrite app_length; simpl; omega.
         * procDec_inv_old; procDec_inv_next 2.
+          destruct x; [discriminate|].
+          destruct x; [reflexivity|discriminate].
+      + kinv_dest_custom procDec_inv_tac; kinv_constr.
+        * apply pgm_init_rq_inv_deq; assumption.
+        * rewrite H2.
+          destruct x; [discriminate|].
+          kinv_regmap_red.
+          rewrite app_length; simpl; omega.
+        * procDec_inv_old; procDec_inv_next 2.
+          destruct x; [discriminate|].
+          destruct x; [reflexivity|discriminate].
           (* END_SKIP_PROOF_OFF *)
   Qed.
 
   Lemma procDec_inv_ok:
     forall o,
-      reachable o (fst pdecInl) ->
+      reachable o pdecInl ->
       procDec_inv o.
   Proof.
     intros; inv H; inv H0.
@@ -489,6 +387,6 @@ Section Invariants.
 End Invariants.
 
 Hint Unfold RqFromProc RsToProc: MethDefs.
-Hint Unfold fifo_rq_rs_inv fifo_inv fifo_empty_inv fifo_not_empty_inv
+Hint Unfold pgm_init_rq_rs_inv fifo_empty_inv fifo_not_empty_inv
        mem_request_inv: InvDefs.
-    
+
