Kami/Ex/ProcDecSC.v
@@ -1,4 +1,4 @@
-Require Import Bool String List.
+Require Import Bool String List Omega.
 Require Import Lib.CommonTactics Lib.ilist Lib.Word.
 Require Import Lib.Struct Lib.FMap Lib.StringEq Lib.Indexer.
 Require Import Kami.Syntax Kami.Semantics Kami.RefinementFacts Kami.Renaming Kami.Wf.
@@ -11,7 +11,7 @@ Require Import Eqdep.
 Set Implicit Arguments.
 
 Section ProcDecSC.
-  Variables addrSize iaddrSize fifoSize instBytes dataBytes rfIdx: nat.
+  Variables addrSize iaddrSize instBytes dataBytes rfIdx: nat.
 
   Variables (fetch: AbsFetch addrSize iaddrSize instBytes dataBytes)
             (dec: AbsDec addrSize instBytes dataBytes rfIdx)
@@ -22,48 +22,116 @@ Section ProcDecSC.
 
   Variable (init: ProcInit iaddrSize dataBytes rfIdx).
 
-  Definition pdec := pdecf fifoSize fetch dec exec init.
+  Definition pdec := pdecf fetch dec exec init.
   Definition pinst := pinst fetch dec exec init.
   Hint Unfold pdec: ModuleDefs. (* for kinline_compute *)
   Hint Extern 1 (ModEquiv type typeUT pdec) => unfold pdec. (* for kequiv *)
   Hint Extern 1 (ModEquiv type typeUT pinst) => unfold pinst. (* for kequiv *)
 
-  Definition pdec_pinst_ruleMap (o: RegsT): string -> option string :=
-    "execToHost" |-> "execToHost";
-      "execNm"     |-> "execNm";
-      "execNmZ"    |-> "execNmZ";
-      "processSt"  |-> "execSt";
-      "processLd"  |-> "execLd"; ||.
-  Hint Unfold pdec_pinst_ruleMap: MethDefs.
+  (* Eval compute in (namesOf (getRules pdec)). *)
+  (* = ["pgmInitRq"%string; "pgmInitRqEnd"%string; "pgmInitRs"%string; "pgmInitRsEnd"%string; *)
+  (*    "reqLd"%string; "reqSt"%string; "repLd"%string; "repLdZ"%string; "repSt"%string; *)
+  (*    "execNm"%string; "execNmZ"%string; "processMem"%string] *)
 
-  Definition pdec_pinst_regMap (r: RegsT): RegsT :=
-    (mlet pcv : (Pc iaddrSize) <- r |> "pc";
-       mlet rfv : (Vector (Data dataBytes) rfIdx) <- r |> "rf";
-       mlet pgmv : (Vector (Data instBytes) iaddrSize) <- r |> "pgm";
-       mlet oev : Bool <- r |> "rsToProc"--"empty";
-       mlet oelv : (Vector (Struct RsToProc) fifoSize) <- r |> "rsToProc"--"elt";
-       mlet odv : (Bit fifoSize) <- r |> "rsToProc"--"deqP";
-       if oev
-       then (["pgm" <- (existT _ _ pgmv)]
-             +["rf" <- (existT _ _ rfv)]
-             +["pc" <- (existT _ _ pcv)])%fmap
-       else
-         let rawInst := pgmv (split2 _ _ pcv) in
-         (["pgm" <- (existT _ _ pgmv)]
-          +["rf" <- (let opc := evalExpr (getOptype _ rawInst) in
-                     if weq opc opLd
-                     then
-                       (existT _ (SyntaxKind (Vector (Data dataBytes) rfIdx))
-                               ((fun a : word rfIdx => if weq a (evalExpr (getLdDst _ rawInst))
-                                                       then oelv odv (RsToProc !! "data")
-                                                       else rfv a)
-                                : (fullType type (SyntaxKind (Vector (Data dataBytes)
-                                                                     rfIdx)))))
-                     else
-                       (existT _ _ rfv))]
-          +["pc" <- (existT _ _ (evalExpr (getNextPc _ rfv pcv rawInst)))])%fmap
-    )%mapping.
-  Hint Unfold pdec_pinst_regMap: MapDefs.
+  (* Eval compute in (namesOf (getRules pinst)). *)
+  (* = ["pgmInit"%string; "pgmInitEnd"%string; "execLd"%string; "execLdZ"%string; "execSt"%string; *)
+  (*    "execNm"%string; "execNmZ"%string] *)
+
+  (* Definition pdec_pinst_ruleMap (o: RegsT): string -> option string := *)
+  (*   "execNm"     |-> "execNm"; *)
+  (*     "execNmZ"    |-> "execNmZ"; *)
+  (*     "processSt"  |-> "execSt"; *)
+  (*     "processLd"  |-> "execLd"; ||. *)
+  (* Hint Unfold pdec_pinst_ruleMap: MethDefs. *)
+
+  (* Eval compute in (namesOf (getRegInits pdec)). *)
+  (* = ["pc"%string; "rf"%string; "pinit"%string; "pinitRq"%string; "pinitRqOfs"%string; *)
+  (*    "pinitRsOfs"%string; "pgm"%string; "stall"%string; "elt.rqFromProc"%string; *)
+  (*    "enqP.rqFromProc"%string; "deqP.rqFromProc"%string; "empty.rqFromProc"%string; *)
+  (*    "full.rqFromProc"%string; "elt.rsToProc"%string; "enqP.rsToProc"%string; *)
+  (*    "deqP.rsToProc"%string; "empty.rsToProc"%string; "full.rsToProc"%string] *)
+
+  (* Eval compute in (namesOf (getRegInits pinst)). *)
+  (* = ["pc"%string; "rf"%string; "pinit"%string; "pinitOfs"%string; "pgm"%string] *)
+
+  Definition drainInst (elt: type (Struct RsToProc))
+             (ofs: type (Bit iaddrSize))
+             (pgmv: type (Vector (Data instBytes) iaddrSize))
+    : fullType type (SyntaxKind (Vector (Data instBytes) iaddrSize)) :=
+    fun w =>
+      if weq w ofs
+      then evalExpr (alignInst _ (elt (RsToProc!!"data")))
+      else pgmv w.
+
+  Fixpoint drainInsts (elts: listEltT (Struct RsToProc) type)
+           (ofs: type (Bit iaddrSize))
+           (pgmv: type (Vector (Data instBytes) iaddrSize))
+    : fullType type (SyntaxKind (Vector (Data instBytes) iaddrSize)) :=
+    match elts with
+    | nil => pgmv
+    | elt :: elts' =>
+      drainInsts elts' (ofs ^+ $1) (drainInst elt ofs pgmv)
+    end.
+
+  Definition pdec_pinst_regRel: RegsT -> RegsT -> Prop.
+  Proof.
+    intros ir sr.
+    kexistv "pc"%string pcv ir (Pc iaddrSize).
+    kexistv "rf"%string rfv ir (Vector (Data dataBytes) rfIdx).
+    kexistv "pinit"%string pinitv ir Bool.
+    kexistv "pgm"%string pgmv ir (Vector (Data instBytes) iaddrSize).
+    kexistnv "rsToProc"--"elt" oeltv ir (listEltK (Struct RsToProc) type).
+    kexistv "pinitRsOfs"%string pinitRsOfsv ir (Bit iaddrSize).
+
+    refine (if pinitv
+            then (match oeltv with
+                  | nil => _
+                  | rs :: oeltv => _
+                  end)
+            else _).
+    - exact (sr = (["pgm" <- (existT _ _ pgmv)]
+                   +["pinitOfs" <- (existT _ _ pinitRsOfsv)]
+                   +["pinit" <- (existT _ _ pinitv)]
+                   +["rf" <- (existT _ _ rfv)]
+                   +["pc" <- (existT _ _ pcv)])%fmap).
+    - set (rawInst := pgmv (split2 _ _ pcv)).
+      exact (sr = (["pgm" <- existT _ _ pgmv]
+                   +["pinitOfs" <- (existT _ _ pinitRsOfsv)]
+                   +["pinit" <- (existT _ _ pinitv)]
+                   +["rf" <- let opc := evalExpr (getOptype _ rawInst) in
+                             if weq opc opLd
+                             then if weq (evalExpr (getLdDst _ rawInst)) $0
+                                  then (existT _ _ rfv)
+                                  else
+                                    (existT
+                                       _ _
+                                       ((fun a => if weq a (evalExpr (getLdDst _ rawInst))
+                                                  then
+                                                    evalExpr
+                                                      (calcLdVal
+                                                         _ (evalExpr
+                                                              (calcLdAddr
+                                                                 _ (evalExpr (getLdAddr type rawInst))
+                                                                 (rfv (evalExpr (getLdSrc type rawInst))))) 
+                                                         (rs Fin.F1)
+                                                         (evalExpr (getLdType _ rawInst)))
+                                                  else rfv a)
+                                        : fullType type (SyntaxKind (Vector (Data dataBytes) rfIdx))))
+                             else (existT _ _ rfv)]
+                   +["pc" <- (existT _ _ (evalExpr (getNextPc _ rfv pcv rawInst)))])%fmap).
+
+    - exact (sr = (["pgm" <- (existT _ _ (drainInsts oeltv pinitRsOfsv pgmv))]
+                   +["pinitOfs" <- (existT _ (SyntaxKind (Bit iaddrSize))
+                                           (pinitRsOfsv ^+ $(List.length oeltv)))]
+                   +["pinit" <- (existT _ (SyntaxKind Bool)
+                                        (if eq_nat_dec
+                                              (#pinitRsOfsv + List.length oeltv)
+                                              (NatLib.pow2 iaddrSize)
+                                         then true else false))]
+                   +["rf" <- (existT _ _ rfv)]
+                   +["pc" <- (existT _ _ pcv)])%fmap).
+  Defined.
+  Hint Unfold pdec_pinst_regRel: MapDefs.
 
   Ltac procDec_inv_old :=
     try match goal with
@@ -78,16 +146,238 @@ Section ProcDecSC.
       | [H: context[Vector_find] |- _] => unfold Vector_find in H; simpl in H
       end.
 
-  Definition decInstConfig :=
-    {| inlining := ITManual;
-       decomposition := DTFunctional pdec_pinst_regMap pdec_pinst_ruleMap;
-       invariants := IVCons procDec_inv_ok IVNil
-    |}.
+  Definition pdecInl := ProcDecInl.pdecInl fetch dec exec init.
 
+  Lemma drainInsts_enq:
+    forall rss rs rsOfs pgmv,
+      drainInsts (listEnq rs rss) rsOfs pgmv =
+      (fun w => if weq w (rsOfs ^+ $ (Datatypes.length rss))
+                then evalExpr (alignInst type (rs Fin.F1))
+                else drainInsts rss rsOfs pgmv w).
+  Proof.
+    unfold listEnq; induction rss; simpl; intros;
+      [rewrite wplus_wzero_1; reflexivity|].
+    rewrite IHrss.
+    rewrite <-wplus_assoc, <-natToWord_plus; reflexivity.
+  Qed.
+  
   Lemma pdec_refines_pinst: pdec <<== pinst.
-  Proof. (* SKIP_PROOF_ON
-    kami_ok decInstConfig procDec_inv_old idtac.
-    END_SKIP_PROOF_ON *) apply cheat.
+  Proof. (* SKIP_PROOF_OFF *)
+
+    (** inlining *)
+    ketrans; [exact (projT2 pdecInl)|].
+
+    (** decomposition *)
+    apply decompositionZeroR_NoRuleMap with (thetaR:= pdec_pinst_regRel);
+      try reflexivity.
+    1: {
+      kdecompose_regrel_init.
+      cbn; rewrite wplus_wzero_1.
+      meq.
+      exfalso; rewrite wordToNat_wzero in e.
+      pose proof (NatLib.pow2_zero iaddrSize); omega.
+    }
+
+    intros.
+    kinv_add procDec_inv_ok.
+    kinvert.
+
+    - kinv_action_dest.
+      kinv_custom procDec_inv_old.
+      kinv_regmap_red.
+      exists None; kinv_constr.
+
+    - kinv_action_dest.
+      kinv_custom procDec_inv_old.
+      kinv_regmap_red.
+      exists None; kinv_constr.
+
+    - kinv_action_dest.
+      kinv_custom procDec_inv_old.
+      kinv_regmap_red.
+      exists None; kinv_constr.
+      kinv_eq.
+      + destruct x1; [discriminate|reflexivity].
+      + rewrite wnot_not_zero_wplusone by assumption.
+        destruct x1; [discriminate|].
+        simpl; rewrite <-Nat.add_assoc; reflexivity.
+      + destruct x1; [discriminate|].
+        simpl; rewrite <-wplus_assoc, <-natToWord_S.
+        reflexivity.
+
+    - kinv_action_dest.
+      kinv_custom procDec_inv_old.
+      kinv_regmap_red.
+      exists None; kinv_constr.
+      apply wnot_zero_wones in e; subst.
+      rewrite wones_pow2_minus_one in H1.
+      simpl; destruct x1 as [|rs ?]; [discriminate|].
+      assert (x1 = nil); subst.
+      { destruct x1; [reflexivity|].
+        destruct pinitRqv; simpl in H1;
+          pose proof (wordToNat_bound pinitRqOfsv); omega.
+      }
+      simpl; kinv_eq.
+      + rewrite wones_pow2_minus_one.
+        find_if_inside; [reflexivity|].
+        elim n; pose proof (NatLib.pow2_zero iaddrSize); omega.
+      + rewrite wones_wneg_one, wplus_comm, wminus_inv; reflexivity.
+        
+    - kinv_action_dest.
+      kinv_custom procDec_inv_old.
+      kinv_regmap_red.
+      exists None; kinv_constr.
+
+    - kinv_action_dest.
+      kinv_custom procDec_inv_old.
+      kinv_regmap_red.
+      exists None; kinv_constr.
+
+    - kinv_action_dest.
+      kinv_custom procDec_inv_old.
+      kinv_regmap_red.
+      exists None; kinv_constr.
+      destruct x; [discriminate|].
+      destruct x; [|discriminate].
+      simpl; subst; kinv_eq; kinv_finish.
+
+    - kinv_action_dest.
+      kinv_custom procDec_inv_old.
+      kinv_regmap_red.
+      exists None; kinv_constr.
+      destruct x; [discriminate|].
+      destruct x; [|discriminate].
+      simpl; subst; kinv_eq; kinv_finish.
+
+    - kinv_action_dest.
+      kinv_custom procDec_inv_old.
+      kinv_regmap_red.
+      exists None; kinv_constr.
+      destruct x; [discriminate|].
+      destruct x; [|discriminate].
+      simpl; subst; kinv_eq; kinv_finish.
+
+    - kinv_action_dest.
+      kinv_custom procDec_inv_old.
+      kinv_regmap_red.
+      exists (Some "execNm"%string); kinv_constr;
+        kinv_eq; kinv_finish.
+
+    - kinv_action_dest.
+      kinv_custom procDec_inv_old.
+      kinv_regmap_red.
+      exists (Some "execNmZ"%string); kinv_constr;
+        kinv_eq; kinv_finish.
+
+    - kinv_action_dest.
+      kinv_custom procDec_inv_old.
+      kinv_regmap_red; kinv_red.
+      destruct pinitv.
+      + specialize (H9 eq_refl); clear H8.
+        kinv_custom procDec_inv_old.
+        kinv_regmap_red.
+        destruct x; [discriminate|].
+        destruct x; [|discriminate].
+        destruct (weq (evalExpr (getLdDst _ (pgmv (split2 2 iaddrSize pcv)))) $0).
+        * exists (Some "execLdZ"%string); kinv_constr; kinv_eq; kinv_finish.
+        * exists (Some "execLd"%string); kinv_constr; kinv_eq; kinv_finish.
+        
+      + specialize (H8 eq_refl); clear H9; kinv_red.
+        destruct (eq_nat_dec (#pinitRsOfsv + Datatypes.length x3)
+                             (NatLib.pow2 iaddrSize - 1)).
+        * exists (Some "pgmInitEnd"%string); kinv_constr; kinv_eq.
+          { simpl; rewrite e.
+            destruct (Nat.eq_dec _ _); [|reflexivity].
+            pose proof (NatLib.pow2_zero iaddrSize); omega.
+          }
+          { cbn; find_if_inside; [reflexivity|].
+            elim n.
+            replace (pinitRsOfsv ^+ $(Datatypes.length x3)) with (wones iaddrSize).
+            { apply wnot_ones. }
+            { rewrite <-natToWord_wordToNat with (w:= pinitRsOfsv).
+              rewrite <-natToWord_plus.
+              rewrite e.
+              apply wones_natToWord.
+            }
+          }
+          { destruct x; [discriminate|].
+            simpl; simpl in H; dest; subst.
+            kinv_eq.
+            do 2 f_equal.
+            rewrite H0; simpl.
+            rewrite <-natToWord_wordToNat with (w:= pinitRsOfsv) at 2.
+            rewrite <-natToWord_plus.
+            f_equal; omega.
+          }
+          { apply eq_sym, drainInsts_enq. }
+          { rewrite e.
+            find_if_inside; [pose proof (NatLib.pow2_zero iaddrSize); omega|].
+            find_if_inside; [reflexivity|].
+            elim n0; unfold listEnq; rewrite app_length; simpl; omega.
+          }
+          { pose proof (NatLib.pow2_zero iaddrSize).
+            rewrite <-natToWord_wordToNat with (w:= pinitRsOfsv).
+            rewrite <-natToWord_plus.
+            unfold listEnq; rewrite app_length; simpl.
+            replace (#pinitRsOfsv + (Datatypes.length x3 + 1))
+              with (NatLib.pow2 iaddrSize) by omega.
+            apply eq_sym, natToWord_pow2.
+          }
+        * assert (#pinitRsOfsv + Datatypes.length x3 < NatLib.pow2 iaddrSize - 1)%nat.
+          { assert (#pinitRsOfsv + Datatypes.length x3 < NatLib.pow2 iaddrSize)%nat.
+            { rewrite <-Nat.add_assoc, Nat.add_comm with (n:= Datatypes.length x) in H0.
+              simpl in H0; rewrite Nat.add_assoc in H0.
+              destruct x; [discriminate|simpl in H0].
+              destruct pinitRqv; simpl in H0;
+                pose proof (wordToNat_bound pinitRqOfsv); omega.
+            }
+            omega.
+          }
+          exists (Some "pgmInit"%string); kinv_constr; kinv_eq.
+          { simpl; destruct (Nat.eq_dec _ _); [omega|reflexivity]. }
+          { cbn; find_if_inside; [|reflexivity].
+            apply wnot_zero_wones in e.
+            rewrite <-natToWord_wordToNat with (w:= pinitRsOfsv) in e.
+            rewrite <-natToWord_plus, wones_natToWord in e.
+            apply natToWord_inj in e; omega.
+          }
+          { destruct x; [discriminate|].
+            simpl; simpl in H; dest; subst.
+            kinv_eq.
+            do 2 f_equal.
+            rewrite H0; simpl.
+            rewrite <-natToWord_wordToNat with (w:= pinitRsOfsv) at 2.
+            rewrite <-natToWord_plus.
+            f_equal; omega.
+          }
+          { apply eq_sym, drainInsts_enq. }
+          { find_if_inside; [omega|].
+            unfold listEnq; rewrite app_length; simpl.
+            find_if_inside; [omega|].
+            reflexivity.
+          }
+          { unfold listEnq; rewrite app_length; simpl.
+            rewrite <-wplus_assoc.
+            rewrite <-natToWord_plus.
+            reflexivity.
+          }
+
+    - kinv_action_dest.
+      kinv_custom procDec_inv_old.
+      kinv_regmap_red; kinv_red.
+      destruct pinitv.
+      + specialize (H9 eq_refl); clear H8.
+        kinv_custom procDec_inv_old.
+        kinv_regmap_red.
+        destruct x; [discriminate|].
+        destruct x; [|discriminate].
+        exists (Some "execSt"%string); kinv_constr; kinv_eq; kinv_finish.
+      + exfalso.
+        specialize (H8 eq_refl); clear H9; kinv_red.
+        destruct x as [|rq ?]; [discriminate|].
+        simpl in H; dest; subst.
+        simpl in H4; discriminate.
+        (* END_SKIP_PROOF_OFF *)
   Qed.
 
 End ProcDecSC.
