Kami/Ex/ProcFetchDecode.v
@@ -141,6 +141,7 @@ Section FetchAndDecode.
                            "op" ::= $$false;
                            "data" ::= $$Default });
       Write "pinitRq" <- $$true;
+      Write "pinitRqOfs" : Bit iaddrSize <- $0;
       Retv
         
     with Rule "pgmInitRs" :=
@@ -169,6 +170,7 @@ Section FetchAndDecode.
       Read pgm <- "pgm";
       Write "pgm" <- #pgm@[#pinitRsOfs <- #inst];
       Write "pinit" <- !#pinit;
+      Write "pinitRsOfs" : Bit iaddrSize <- $0;
       Retv
 
     (** Phase 2: execute the program [pinit == true] *)
